

Q1 Linear equations.

$$4x + y + z = 6$$

$$x + 3y + z = 5$$

$$x + y + 2z = 4$$

a) Backward substitution

$$\begin{bmatrix} 4 & 1 & 1 & 6 \\ 1 & 3 & 1 & 5 \\ 1 & 1 & 2 & 4 \end{bmatrix}$$

Converted to matrix form

 $R_1 \leftrightarrow R_2$  swapping (ERO 1)

$$\begin{bmatrix} 1 & 3 & 1 & 5 \\ 4 & 1 & 1 & 6 \\ 1 & 1 & 2 & 4 \end{bmatrix}$$

row operations

$$R_2 \rightarrow R_2 - 4R_1$$

$$\begin{bmatrix} 4 & 1 & 1 & 6 \end{bmatrix} - 4 \begin{bmatrix} 1 & 3 & 1 & 5 \end{bmatrix}$$

$$\begin{bmatrix} 4 & 1 & 1 & 6 \end{bmatrix} - \begin{bmatrix} 4 & 12 & 4 & 20 \end{bmatrix}$$

$$\begin{bmatrix} 0 & -11 & -3 & -14 \end{bmatrix} - R_2 \text{ row answer}$$

$$R_3 \rightarrow R_3 - R_1$$

$$\begin{bmatrix} 1 & 1 & 2 & 4 \end{bmatrix} - \begin{bmatrix} 1 & 3 & 1 & 5 \end{bmatrix} = \begin{bmatrix} 0 & -2 & 1 & -1 \end{bmatrix}$$

(2)

substitute  $R_2$  and  $R_3$  in original matrix

20259605129

$$\begin{bmatrix} 1 & 3 & 1 & 5 \\ 0 & -11 & -3 & -14 \\ 0 & -2 & 1 & -1 \end{bmatrix}$$

$$R_3 \rightarrow R_3 - \frac{2}{11} R_2$$

$$\begin{bmatrix} 0 & -2 & 1 & -1 \end{bmatrix} - \frac{2}{11} \begin{bmatrix} 0 & -11 & -3 & -14 \end{bmatrix}$$

$$\begin{bmatrix} 0 & -2 & 1 & -1 \end{bmatrix} - \begin{bmatrix} 0 & -2 & -\frac{6}{11} & -\frac{28}{11} \end{bmatrix}$$

$$= \begin{bmatrix} 0 & 0 & 1 - \frac{6}{11} & -1 - \frac{28}{11} \end{bmatrix}$$

$$= \begin{bmatrix} 0 & 0 & \frac{17}{11} & \frac{17}{11} \end{bmatrix}$$

replace  $R_3$  in original

$$\begin{bmatrix} 1 & 3 & 1 & 5 \\ 0 & -11 & -3 & -14 \\ 0 & 0 & \frac{17}{11} & \frac{17}{11} \end{bmatrix}$$

Backward substitution

$$\frac{17}{11} z = \frac{17}{11}$$

$$\boxed{z = 1} //$$

$$x + 3y + 2z = 5$$

$$0 - 11y - 3z = -14$$

$$0 - 11y - 3x = -14$$

$$-11y = -14 + 3$$

$$\boxed{y = 1}$$

From  $R_1$

$$4x + y + z = 6$$

$$4x + 1 + 1 = 6$$

$$4x = 6 - 2$$

$$\boxed{x = 1}$$

$$\boxed{x = 1, y = 1, z = 1}$$

b) Eigen decomposition method

$$A = \begin{bmatrix} 4 & 1 & 1 \\ 1 & 3 & 1 \\ 1 & 1 & 2 \end{bmatrix} \quad b = \begin{bmatrix} 6 \\ 5 \\ 4 \end{bmatrix}$$

Its a symmetric

$$A = A^T$$



(A)

$$|A - \lambda I| = 0$$

$$\lambda^3 - S_1 \lambda^2 + S_2 \lambda - S_3 = 0$$

$S_1$  = sum of diagonal matrix

$$4 + 3 + 2 = 9$$

$S_2$  = sum of minus of diagonal elements.

$$\begin{vmatrix} 3 & 1 \\ 1 & 2 \end{vmatrix} + \begin{vmatrix} 4 & 1 \\ 1 & 2 \end{vmatrix} + \begin{vmatrix} 4 & 1 \\ 1 & 3 \end{vmatrix}$$

$$= 6 - 1 + 8 - 1 + 12 - 1$$

$$S_2 = 23$$

$$S_3 = |A|$$

$$= 4 \begin{vmatrix} 3 & 1 \\ 1 & 2 \end{vmatrix} - 1 \begin{vmatrix} 1 & 1 \\ 1 & 2 \end{vmatrix} + 1 \begin{vmatrix} 1 & 3 \\ 1 & 1 \end{vmatrix}$$

$$= 4(6 - 1) - 1(2 - 1) + 1(1 - 3)$$

$$= 17$$

$$\lambda^3 - 9\lambda^2 + 23\lambda - 17 = 0$$

solving above cubic ic calc equation mode

$$\lambda_1 = 5.214319743$$

$$\lambda_2 = 2.460811127$$

$$\lambda_3 = 1.324869129$$

5)  $A = \text{Eigen vector } \lambda_1 = 5.214319743$

$$(A - \lambda I)v = 0$$

$$= \begin{pmatrix} 4 - 5.214319743 & 1 & 1 \\ 1 & 3 - 5.214319743 & 1 \\ 1 & 1 & 2 - 5.214319743 \end{pmatrix}$$

$$= \begin{pmatrix} -1.214319743 & 1 & 1 \\ 1 & -2.214319743 & 1 \\ 1 & 1 & -3.214319743 \end{pmatrix}$$

$$\text{let } v = \begin{pmatrix} x \\ y \\ z \end{pmatrix}$$

$$-1.214319743x + y + z = 0$$

$$x - 2.214319743y + z = 0$$

$$x + y - 3.214319743z = 0$$

Solve the above equation

$$y = 1.214319743 - z$$

①

Suresh babu V

/ /

2025AB 05129

$$x - 2.214319743(1.214319743x - z) + z = 0$$

$$3.214319742 = 1.68889218x$$

$$z = 0.524275609x$$

$$y = 1.214319743x - 0.524275609x$$

$$y = 0.6888921821x$$

Eigen vector  $V_1 (x, 0.6888921821x, 0.524275609x)$

$$\|V_1\| = \sqrt{1^2 + 0.6888921821^2 + 0.524275609^2}$$

$$= 1.32312001$$

$$V_1 = \frac{1}{\|V_1\|} = \frac{1}{1.32312001} (1, 0.6888921821, 0.524275609)$$

$$V_1 = (0.7557893408, 0.5206573481, 0.3971125498)$$

Eigen vector  $\lambda_2 = 2.460811127$

$$(A - \lambda_2 I)v = 0 = \begin{pmatrix} 4 - 2.460811127 & 0 & 0 \\ 0 & 3 - 2.460811127 & 0 \\ 0 & 0 & 2 - 2.460811127 \end{pmatrix}$$



(7)

suresh babu V

\_/\_/\_

20250605129

$$= 1.539188673$$

1

$$0.539188673$$

1

1

$$-0.460811127$$

solve equation by substituting

$$1) 1.539188673x + y + z = 0$$

$$2) x + 0.539188673y + z = 0$$

$$3) x + y - 0.460811127z = 0$$

$$x + 0.539188673(1.539188673x - z) + z = 0$$

$$x - 0.829135138x - 0.539188673z + z = 0$$

$$0.1700864862x + 0.460811127z = 0$$

$$z = \frac{-0.1700864862x}{0.460811127}$$

$$z = -0.3691023854x$$

$$y = z - 1.539188673x$$

$$= -0.3691023854x - 1.539188673x$$

$$= -1.170086488x$$

$$V_2 = (x, -1.170086488x, -0.3691023854x)$$

$$\|V_2\| = \sqrt{1^2 + (-1.170086488)^2 + (-0.3691023854)^2}$$

$$= 1.582826257$$

$$V_2 = (0.6317812808, -0.7392387401, -0.2331919778)$$

⑧

suresh baba V

\_/\_/\_

2023 ab 05/29

Eigen vector corresponding to  $\lambda_3 = 1.324869129$ 

$$(A - \lambda_3 I)V = \begin{pmatrix} 4 - 1.324869129 & 1 & 1 \\ 1 & 3 - 1.324869129 & 1 \\ 1 & 1 & 2 - 1.324869129 \end{pmatrix}$$

$$= \begin{pmatrix} 2.675130871 & 1 & 1 \\ 1 & 1.675130871 & 1 \\ 1 & 1 & 0.675130871 \end{pmatrix}$$

substituting equation

- 1.)  $2.675130871x + y + z = 0$
- 2.)  $x + 1.675130871y + z = 0$
- 3.)  $x + y + 0.675130871z = 0$

$$x + 1.675130871(-2.675130871x - z) + z = 0$$

$$x - 4.481194182 - 1.657130871z + z = 0$$

$$z = \frac{3.481194182}{-0.675130871} = -5.15632517x$$

$$y = -z - 2.675130871x$$

$$= 5.15632517x - 2.675130871x =$$

$$= 2.481194303x$$



9

Suryash babu v

\_/\_/\_

20259605129

$$V_3 (x, 2.48119403x, -5.15632174x)$$

$$\begin{aligned} \|V_3\| &= \sqrt{1^2 + 2.48119403^2 + (-5.15632174)^2} \\ &= 5.808959844 \end{aligned}$$

$$V_3 = (0.172147859, 0.427132287, -0.8876503389)$$

Eigen vector and eigen decomposition

$$A = PDP$$

$$P = [V_1 \ V_2 \ V_3], \quad D = \text{diag}(\lambda_1, \lambda_2, \lambda_3)$$

$$\text{set } x = Pz$$

$$Ax = PDP^T(Pz)$$

$$P^T P D z = P^T b$$

$$Dz = P^T b$$

$$z = D^{-1}(P^T b), \quad x = Pz$$

$$\text{hence } y = P^T b \quad (y_i = v_i^T b)$$

$$\begin{aligned} y_1 = v_1^T b &= (0.7557893408 \times 6) + (0.5206573681 \times 5) \\ &\quad + (0.397112548 \times 4) \end{aligned}$$

(10)

Suresh babu V  
2025 05 05 129

$$= 8.726473077$$

$$y_2 = V_2^T b = (0.6317812808 \times 6) + (-0.7392387401 \times 5) + (-0.233199778 \times 4)$$

$$= -0.83822394$$

$$y_3 = V_3^T b = (0.1721478596) + (0.42713228 \times 5) + (-0.8876503389 \times 4)$$

$$= -0.3820527666$$

$$z_i = y_i / \lambda_i$$

$$z_1 = y_1 / \lambda_1 = \frac{8.726473077}{5.214319743} = 1.673559257$$

$$z_2 = y_2 / \lambda_2 = \frac{-0.88822394}{2.460811127} = -0.3406494431$$

$$z_3 = y_3 / \lambda_3 = \frac{0.3820527666}{1.324869129} = 0.2883701931$$

$$x = p_2 = z_1 V_1 + z_2 V_2 + z_3 V_3$$

$$x = 1.673559257 \begin{pmatrix} 0.75557893408 \\ 0.5206573681 \\ 0.3971125498 \end{pmatrix}$$

$$- 0.3406494431 \begin{pmatrix} 0.6317812808 \\ 0.7392387401 \\ -0.233199778 \end{pmatrix}$$



(11)

Suresh babu v

2025 9605129

$$+ 0.2883701931 \begin{pmatrix} -0.172147859 \\ -0.427132287 \\ 0.8876503887 \end{pmatrix}$$

$$= \begin{pmatrix} 1.264858248 \\ 0.8713509581 \\ 0.6645913838 \end{pmatrix} + \begin{pmatrix} -0.2152159415 \\ 0.2518212651 \\ 0.07943671737 \end{pmatrix} + \begin{pmatrix} -0.04964231134 \\ -0.1231722201 \\ 0.2559719141 \end{pmatrix}$$

$$x = \begin{pmatrix} 0.9999999952 \\ 1.0000000003 \\ 1.0000000015 \end{pmatrix}$$

Approximated

$$x = \begin{pmatrix} 1 \\ 1 \\ 1 \end{pmatrix}$$

c.) Cholesky decomposition  $Ax = b$ 

$$Ax = b \begin{pmatrix} 4 & 1 & 1 \\ 1 & 3 & 1 \\ 1 & 1 & 2 \end{pmatrix} \begin{pmatrix} 1 \\ 1 \\ 1 \end{pmatrix} = \begin{pmatrix} 6 \\ 5 \\ 4 \end{pmatrix} = b$$



(12)

As matrix A is symmetric, cholesky factorization can be applied.

$A = LL^T$ , L = lower triangular matrix

$$L = \begin{pmatrix} l_{11} & 0 & 0 \\ l_{21} & l_{22} & 0 \\ l_{31} & l_{32} & l_{33} \end{pmatrix}$$

$$LL^T = \begin{pmatrix} l_{11} & 0 & 0 \\ l_{21} & l_{22} & 0 \\ l_{31} & l_{32} & l_{33} \end{pmatrix} \begin{pmatrix} l_{11} & l_{21} & l_{31} \\ 0 & l_{22} & l_{32} \\ 0 & 0 & l_{33} \end{pmatrix}$$

$$= \begin{pmatrix} l_{11}^2 & l_{11}l_{21} & l_{11}l_{31} \\ l_{21}l_{11} & l_{11}^2 + l_{22}^2 & l_{21}l_{31} + l_{22}l_{32} \\ l_{31}l_{11} & l_{32} + l_{33}l_{22} & l_{31}^2 + l_{32}^2 + l_{33}^2 \end{pmatrix}$$

$$= \begin{pmatrix} 4 & 1 & 1 \\ 1 & 3 & 1 \\ 1 & 1 & 2 \end{pmatrix}$$

(13)

suresh babu v

\_/\_/\_

2025 ab 05129

Substitute  $q_i$  in  $l_{ij}$ 

$$q_{11} = l_{11}^2 = 4$$

$$l_{11} = 2$$

$$q_{21} = l_{21} l_{11} = 1$$

$$l_{21} = \frac{1}{2}$$

$$q_{31} = l_{31} l_{11} = 1$$

$$l_{31} = \frac{1}{2}$$

$$q_{22} = l_{21}^2 + l_{22}^2 = 3$$

$$l_{22}^2 = 3 - \left(\frac{1}{2}\right)^2 = 3 - \frac{1}{4} = \frac{11}{4}$$

$$l_{22} = \frac{\sqrt{11}}{2}$$

$$q_{32} = l_{31} l_{21} + l_{32} l_{22} = 1$$

$$l_{32} = \frac{1 - l_{31} l_{21}}{l_{22}} = \frac{1 - 1/4}{\frac{\sqrt{11}}{2}}$$

$$= \frac{3}{2\sqrt{11}}$$



(14)

$$a_{33} = l_{31}^2 + l_{32}^2 + l_{33}^2 = 2$$

$$l_{32}^2 = 2 - \frac{1}{4} - \frac{9}{44}$$

$$l_{32}^2 = \frac{88 - 11 - 9}{44}$$

$$l_{32}^2 = \frac{68}{44} = \frac{17}{11}$$

$$l_{32} = \sqrt{17/11}$$

hence  $L = \begin{pmatrix} 2 & 0 & 0 \\ \frac{1}{2} & \frac{\sqrt{11}}{2} & 0 \\ \frac{1}{2} & \frac{3}{2\sqrt{11}} & \sqrt{17/11} \end{pmatrix}$

Apply Forward substitution  $Ly = b$

Backward substitution  $L^T x = y$

$$L = 1) \quad 2y_1 = 6$$

$$y_1 = \frac{6}{2} = 3$$

$$2) \quad \frac{1}{2}y_1 + \frac{\sqrt{11}}{2}y_2 = 5$$

$$3) \quad \frac{1}{2}y_1 + \frac{3}{2\sqrt{11}}y_2 + \sqrt{\frac{17}{11}}y_3 = 4$$



(15)

suresh babu v

\_/\_/\_  
2025 ab05129

$$\frac{1}{2}(3) + \frac{\sqrt{11}}{2} y_2 = 5$$

$$\frac{\sqrt{11}}{2} y_2 = 5 - \frac{3}{2}$$

$$y_2 = \frac{7/2}{\frac{\sqrt{11}}{2}} = \frac{7}{\sqrt{11}}$$

third eq

$$\frac{1}{2}(5) + \frac{3}{2\sqrt{11}} \cdot \frac{7}{\sqrt{11}} + \sqrt{17/11} y_3 = 4$$

$$\frac{3}{2} + \frac{21}{22} + \sqrt{17/11} y_3 = 4$$

$$\sqrt{17/11} y_3 = 4 - \frac{27}{11}$$

$$y_3 = 4 - \frac{27}{11} \times \sqrt{11/17}$$

$$= \frac{17}{11} \times \sqrt{11/17}$$

$$y_3 = \sqrt{17/11}$$

$$y = \begin{pmatrix} 3 \\ 7/\sqrt{11} \\ \sqrt{17/11} \end{pmatrix}$$

(16)

suresh baba v

2025/05/29

hence  $L^T =$ 

$$L^T = \begin{pmatrix} 2 & \frac{1}{2} & \frac{1}{2} \\ 0 & \frac{\sqrt{11}}{2} & \frac{3}{2}\sqrt{11} \\ 0 & 0 & \sqrt{17/11} \end{pmatrix}$$

Apply in the equation

$$1) 2x_1 + \frac{1}{2}x_2 + \frac{1}{2}x_3 = 3$$

$$2) \frac{\sqrt{11}}{2}x_2 + \frac{3}{2\sqrt{11}}x_3 = \frac{7}{\sqrt{11}}$$

$$3) \sqrt{17/11}x_3 = \sqrt{17/11} \Rightarrow x_3 = 1$$

 $x_3 = 1$ , apply in 2

$$\frac{\sqrt{11}}{2}x_2 + \frac{3}{2\sqrt{11}} \cdot 1 = \frac{7}{\sqrt{11}}$$

multiply bot sides by  $\frac{2}{\sqrt{11}}$ 

$$x_2 + \frac{3}{2\sqrt{11}} \times \frac{2}{\sqrt{11}} = \frac{7}{\sqrt{11}} \cdot \frac{2}{\sqrt{11}}$$

$$x_2 + \frac{6}{22} = \frac{14}{11}$$

$$x_2 = \frac{14}{11} - \frac{6}{22} = 1$$

substitute in equation 1

$$2x_1 + \frac{1}{2} \cdot 1 + \frac{1}{2} \cdot 1 = 3$$

 ~~$x_1 = 1$~~



(17)

Suresh babu

\_/\_/\_

2025 9b 05129

$$2x_1 + 1 = 3$$

$$x_1 = 1$$

$$y = 1$$

$$(x_1 = 1, x_2 = 1, x_3 = 1)$$

as per equation.

$$(x = 1, y = 1, z = 1)$$

D) compare All three methods.

Method	Remarks	Cost
Backward Substitution	Suitable for small systems	Low
Eigen - decomposition	It requires lot of compute, hence expensive	High
cholesky decomposition	For symmetric positive it is best method.	very efficient

cholesky decomposition is best since

the computational steps is very less and efficient,



(12)

Q2. Inner product of  $\mathbb{R}^4$  :

$$(x, y) = x^T M y$$

$$M = \begin{pmatrix} 2 & -1 & 0 & 0 \\ -1 & 3 & 0 & 0 \\ 0 & 0 & 4 & 1 \\ 0 & 0 & 1 & 2 \end{pmatrix}$$

vectors

$$u = \begin{pmatrix} 1 \\ 2 \\ 0 \\ 1 \end{pmatrix}$$

$$v = \begin{pmatrix} 0 \\ 1 \\ 1 \\ 1 \end{pmatrix}$$

$$w = \begin{pmatrix} 1 \\ 0 \\ 2 \\ 0 \end{pmatrix}$$

a) verify inner product

$$M^T = \begin{pmatrix} 2 & -1 & 0 & 0 \\ -1 & 3 & 0 & 0 \\ 0 & 0 & 4 & 1 \\ 0 & 0 & 1 & 2 \end{pmatrix}$$

a)  $M = M^T$  which is symmetric.hence  $(x, y) = x^T M y = y^T M x = (y, x) //$



(19)

b)

20250605129

Positive definiteness:  $(x, x) = x^T M x > 0$  for  $x \neq 0$ 

Apply block diagonal

$$B_1 = \begin{pmatrix} 2 & -1 \\ -1 & 3 \end{pmatrix} \quad B_2 = \begin{pmatrix} 4 & 1 \\ 1 & 2 \end{pmatrix}$$

$$\det(B_1) = (6-1) = 5 > 0, \quad \det(B_2) = (8-1) = 7 > 0$$

c) no need check bilinearity, since built in  $x^T M y$ Based on  $a, b, c, \langle \cdot, \cdot \rangle$  is an inner product on  $\mathbb{R}^4$ B. compute the inner products  $(u, v), (u, w), (v, w)$ Find  $m_v, m_w$ 

$$(x, y) = x^T (m_y)$$

$$m_v = \begin{bmatrix} 2(0) + (-1)(1) + 0 \times 0 + 0 \times 0 \\ 1(0) + (3)(1) + 0 + 0 \\ 0 + 0 + 4 \times 1 + 1 \times 1 \\ 0 + 0 + 1 \times 1 + 2 \times 1 \end{bmatrix} = \begin{pmatrix} -1 \\ 3 \\ 5 \\ 3 \end{pmatrix}$$



(20)

suresh babu V

2025 9b 05129

the inner products

$$(u, v) = u^T (Mv)$$

$$u = \begin{pmatrix} 1 \\ 2 \\ 0 \\ 1 \end{pmatrix}$$

$$u^T = (1 \ 2 \ 0 \ 1)$$

$$(u, v) = u^T (Mv) = \begin{pmatrix} 1 & 2 & 0 & 1 \end{pmatrix} \begin{pmatrix} -1 \\ 3 \\ 5 \\ 3 \end{pmatrix}$$

$$= -1 + 6 + 0 + 3$$

$$(u, v) = 8$$

$$(u, w) = u^T M w$$

$$= \begin{pmatrix} 1 & 2 & 0 & 1 \end{pmatrix} \begin{pmatrix} 2 & -1 & 0 & 0 \\ -1 & 3 & 0 & 0 \\ 0 & 0 & 1 & 1 \\ 0 & 0 & 1 & 2 \end{pmatrix} \begin{pmatrix} 1 \\ 0 \\ 2 \\ 0 \end{pmatrix}$$

(21)

Surpsh babu v

/ / /

2025 ab 05129

$$= \begin{pmatrix} 1 & 2 & 0 & 1 \end{pmatrix} \begin{bmatrix} 2 \times 1 + -1 \times 0 + 0 + 0 \\ -1 \times 1 + 3 \times 0 + 0 + 0 \\ 0 + 0 + 4 \times 2 + 1 \times 0 \\ 0 \times 1 + 0 + 1 \times 2 + 2 \times 0 \end{bmatrix}$$

$$= \begin{pmatrix} 1 & 2 & 0 & 1 \end{pmatrix} \begin{pmatrix} 2 \\ -1 \\ 8 \\ 2 \end{pmatrix}$$

$$= 2 + (-2) + 0 + 2$$

$$\langle u, w \rangle = 2$$

$$\langle u, w \rangle = u^T M w = 2 //$$

$$v w = v^T M w$$

$$= \begin{pmatrix} 0 & 1 & 1 & 1 \end{pmatrix} \begin{pmatrix} 2 \\ -1 \\ 8 \\ 2 \end{pmatrix}$$

$$= 0 + (-1) + 8 + 2$$

$$v w = v^T M w = 9 //$$



c) norms  $\|u\|$ ,  $\|v\|$ ,  $\|w\|$

with respect to the given inner product

$$\|x\| = \sqrt{(x, x)}$$

$$(x, x) = x^T M x$$

$$(u, u) = u^T M u$$

$$u = \begin{pmatrix} 1 \\ 2 \\ 0 \\ 1 \end{pmatrix} \quad u^T = [1 \ 2 \ 0 \ 1]$$

$$= \begin{bmatrix} 1 & 2 & 0 & 1 \end{bmatrix} \begin{bmatrix} 2 & -1 & 5 & 0 \\ -1 & 3 & 0 & 0 \\ 0 & 0 & 1 & 1 \\ 0 & 0 & 1 & 2 \end{bmatrix} \begin{bmatrix} 1 \\ 2 \\ 0 \\ 1 \end{bmatrix}$$

$$= [1 \ 2 \ 0 \ 1] \begin{bmatrix} 2 \times 1 + -1 \times 2 + 0 + 0 \\ -1 + 6 + 0 + 0 \\ 0 + 0 + 0 + 1 \\ 0 + 0 + 0 + 2 \end{bmatrix}$$

$$= [1 \ 2 \ 0 \ 1] \begin{bmatrix} 0 \\ 5 \\ 1 \\ 2 \end{bmatrix}$$

$$= [1 \times 0 + 5 \times 2 + 0 + 1 \times 2]$$

$$= 12$$

$$(u, v) = \|u\|^2 = 12$$

$$\|u\| = \sqrt{12} (3 + 2 + 0) = \sqrt{12}$$

$$\|u\| = 2\sqrt{3}$$

$$(u, v) = V^T M V$$

$$V = \begin{pmatrix} 0 \\ 1 \\ 1 \\ 1 \end{pmatrix} \quad V^T = \begin{bmatrix} 0 & 1 & 1 & 1 \end{bmatrix}$$

$$= \begin{pmatrix} 0 & 1 & 1 & 1 \end{pmatrix} \begin{pmatrix} 2 & -1 & 0 & 0 \\ -1 & 3 & 0 & 0 \\ 0 & 0 & 4 & 1 \\ 0 & 0 & 1 & 2 \end{pmatrix} \begin{pmatrix} 0 \\ 1 \\ 1 \\ 1 \end{pmatrix}$$

$$= \begin{pmatrix} 0 & 1 & 1 & 1 \end{pmatrix} \begin{pmatrix} 2 \times 0 + -1 + 0 + 0 \\ 0 + 3 + 0 + 0 \\ 0 + 0 + 4 + 1 \\ 0 + 0 + 1 + 2 \end{pmatrix}$$



$$= (0 \ 1 \ 1 \ 1) \begin{pmatrix} -1 \\ 3 \\ 5 \\ 3 \end{pmatrix}$$

$$VV = (0 + 3 + 5 + 3)$$

$$VV = 11$$

$$\boxed{\|V\| = \sqrt{11}}$$

$$(w, w) = W^T M W$$

$$W = \begin{pmatrix} 1 \\ 0 \\ 2 \\ 0 \end{pmatrix} \quad W^T = \begin{bmatrix} 1 & 0 & 2 & 0 \end{bmatrix}$$

$$(w, w) = \begin{pmatrix} 1 \\ 0 \\ 2 \\ 0 \end{pmatrix}^T \begin{pmatrix} 2 & -1 & 0 & 0 \\ -1 & 3 & 0 & 0 \\ 0 & 0 & 4 & 1 \\ 0 & 0 & 1 & 2 \end{pmatrix} \begin{pmatrix} 1 & 0 & 2 & 0 \end{pmatrix}$$

$$(w, w) = \begin{pmatrix} 1 \\ 0 \\ 2 \\ 0 \end{pmatrix}^T \begin{pmatrix} 2+0+0+0 \\ -1+0+0+0 \\ 0+0+8+0 \\ 0+0+2+0 \end{pmatrix}$$

$$= \begin{pmatrix} 1 \\ 0 \\ 2 \\ 0 \end{pmatrix}^T \begin{pmatrix} 2 \\ -1 \\ 8 \\ 2 \end{pmatrix}$$

$$= (1 \ 0 \ 2 \ 0) \begin{pmatrix} 2 \\ -1 \\ 8 \\ 2 \end{pmatrix}$$

$$= 2 + 0 + 16 + 0$$

$$(w, w) = 18$$

$$\|w\| = \sqrt{18}$$

$$\boxed{\|w\| = 3\sqrt{2}}$$



26

$$\|u\| = 2\sqrt{3}, \quad \|v\| = \sqrt{11}, \quad \|w\| = 3\sqrt{2}$$

d)  $u, v, w$  are linearly independent

definition used

$$\alpha u + \beta v + \gamma w = 0$$

$$\alpha = \beta = \gamma = 0$$

Given vectors

$$u = \begin{pmatrix} 1 \\ 2 \\ 0 \\ 1 \end{pmatrix}, \quad v = \begin{pmatrix} 0 \\ 1 \\ 1 \\ 1 \end{pmatrix}, \quad w = \begin{pmatrix} 1 \\ 0 \\ 2 \\ 0 \end{pmatrix}$$

$$\alpha \begin{pmatrix} 1 \\ 2 \\ 0 \\ 1 \end{pmatrix} + \beta \begin{pmatrix} 0 \\ 1 \\ 1 \\ 1 \end{pmatrix} + \gamma \begin{pmatrix} 1 \\ 0 \\ 2 \\ 0 \end{pmatrix} = \begin{pmatrix} 0 \\ 0 \\ 0 \\ 0 \end{pmatrix}$$

First co-ordinate

$$\alpha(1) + \beta(0) + \gamma(1) = 0$$

$$\alpha + \gamma = 0$$



second co-ordinate

$$\alpha(2) + \beta(1) + \gamma(0) = 0$$

$$2\alpha + \beta = 0$$

Third co-ordinate

$$\alpha \cdot 0 + \beta + \gamma(2) = 0$$

$$\beta + 2\gamma = 0$$

Fourth co-ordinate

$$\alpha x + \beta + \gamma x = 0$$

$$\alpha + \beta = 0$$

let  $\alpha = 0$

equation 1  $\alpha + \gamma = 0$ ,  $0 + \gamma = 0$

ie  $\gamma = 0$  (gamma is zero)

equation 2

$$2\alpha + \beta = 0$$

$$2 \times 0 + \beta = 0$$

ie  $\beta = 0$  (beta is zero)



hence

$$\alpha = \beta = \gamma = 0$$

Therefore  $u, v, w$  are linearly independent in  $\mathbb{R}^4$

e) Gram Schmidt  $u, v, w$  produce an orthogonal set

orthogonal vectors  $a_1, a_2, a_3$

normalized orthonormal vectors  $e_1, e_2, e_3$

$$a_1 = u$$

$$\text{Inner product } (a_1, a_1) = u, u = 12$$

$$e_1 = \frac{a_1}{\sqrt{(a_1, a_1)}} = \frac{1}{\sqrt{12}} \begin{bmatrix} 1 \\ 2 \\ 0 \\ 1 \end{bmatrix} = \frac{1}{2\sqrt{3}} \begin{bmatrix} 1 \\ 2 \\ 0 \\ 1 \end{bmatrix}$$

Step 2  $a_2 = \text{Projection of } v \text{ into } a_1$

$$e_2 = \frac{u_2}{\|u_2\|}$$

$$u_2 = v - \frac{(v, u_1)}{(u_1, u_1)} u_1$$

$$\text{Ans) } \alpha_1(v) = \frac{\langle v, a_1 \rangle}{\langle a_1, a_1 \rangle} a_1 = \frac{\langle v, u \rangle}{\langle u, u \rangle}$$

$$= \frac{8}{12} u$$

$$= \frac{2}{3} u$$

$$a_2 = v - \frac{2}{3} u$$

$$= \begin{pmatrix} 0 \\ 1 \\ 1 \\ 1 \end{pmatrix} - \frac{2}{3} \begin{pmatrix} 1 \\ 2 \\ 0 \\ 1 \end{pmatrix}$$

$$= \begin{pmatrix} 0 \\ 1 \\ 1 \\ 1 \end{pmatrix} - \begin{pmatrix} \frac{2}{3} \\ \frac{4}{3} \\ 0 \\ \frac{2}{3} \end{pmatrix}$$

$$a_2 = \begin{pmatrix} -2/3 \\ -1/3 \\ 1 \\ 1/3 \end{pmatrix}$$



$$\text{now } (a_2, a_2) = a_2^T M a_2$$

$$= \begin{pmatrix} -2/3 & -1/3 & 1 & 1/3 \end{pmatrix} \begin{pmatrix} 2 & -1 & 0 & 0 \\ -1 & 3 & 0 & 0 \\ 0 & 0 & 4 & 1 \\ 0 & 0 & 1 & 2 \end{pmatrix} \begin{pmatrix} -2/3 \\ -1/3 \\ 1 \\ 4/3 \end{pmatrix}$$

$$= \begin{pmatrix} -2/3 & -1/3 & 1 & 1/3 \end{pmatrix} \begin{pmatrix} 2 \times \frac{-2}{3} + -1 \times \frac{-1}{3} + 0 + 0 \\ -1 \times \frac{-2}{3} + 3 \times \frac{-1}{3} + 0 + 0 \\ 0 + 0 + 4 + 1 \times \frac{1}{3} \\ 0 + 0 + 1 + 2 \times \frac{1}{3} \end{pmatrix}$$

$$= \begin{pmatrix} -\frac{2}{3} & -\frac{1}{3} & 1 & \frac{1}{3} \end{pmatrix} \begin{pmatrix} -1 \\ -\frac{1}{3} \\ \frac{13}{3} \\ \frac{5}{3} \end{pmatrix}$$

$$= \left( -\frac{2}{3} \times -1 + \frac{-1}{3} \times -\frac{1}{3} + 1 \times \frac{13}{3} + \frac{1}{3} \times \frac{5}{3} \right)$$

$$= \frac{2}{3} + \frac{1}{9} + \frac{13}{3} + \frac{5}{9} = \frac{17}{3}$$

$$= \frac{17}{3}$$

(31)

Suresh babu

\_/\_/\_

2023 06 05 12 9

$$\langle a, a_2 \rangle = 17/3$$

$$\|a_2\| = \sqrt{17/3}$$

$$p_2 = \frac{a_2}{\|a_2\|} = \frac{a_2}{\sqrt{17/3}}$$

$$p_2 = \sqrt{3/17} \begin{bmatrix} -2/3 \\ -1/3 \\ 1 \\ 1/3 \end{bmatrix}$$

$a_3$  is result of orthogonalization of  $w$  against  $a, a_2$

$$a_3 = w - \text{proj}_{a_1}(w) - \text{proj}_{a_2}(w)$$

$$\text{proj}_{a_1}(w) = \frac{(w, a_1)}{(a_1, a_1)} a_1 = \frac{w, u}{12} u = \frac{2}{12} u$$

$$= \frac{1}{6} u$$



(32)

Suresh babu V

\_/\_/\_

2025 9505129

$$(w, a_2) = w^T (M a_2)$$

$$= \begin{pmatrix} 1 & 0 & 2 & 0 \end{pmatrix} \begin{pmatrix} -1 \\ -1/3 \\ 13/3 \\ 5/3 \end{pmatrix} = \|w\|$$

$$= (1 \times -1 + 0 + 2 \times \frac{13}{3} + 0)$$

$$= (-1 + 0 + \frac{26}{3} + 0)$$

$$= \frac{23}{3}$$

$$\text{proj}_{a_2}(w) = \frac{(w, a_2)}{a_2 \cdot a_2} a_2$$

$$= \frac{23/3}{17/3} \cdot a_2$$

$$= \frac{23}{17} \begin{pmatrix} -2/3 \\ -1/3 \\ 1 \\ 1/3 \end{pmatrix}$$

$$a_3 = w - \text{proj}_{a_1}(w) - \text{proj}_{a_2}(w)$$

(33)

Suresh babu

\_/\_/\_

2025/05/29

$$q_3 = \begin{pmatrix} 1 \\ 0 \\ 2 \\ 0 \end{pmatrix} - \frac{1}{6} \begin{pmatrix} 1 \\ 2 \\ 0 \\ 1 \end{pmatrix} - \frac{23}{17} \begin{pmatrix} -2 \\ 5 \\ -1 \\ 3 \end{pmatrix}$$

$$= \begin{pmatrix} 1 \\ 0 \\ 2 \\ 0 \end{pmatrix} - \begin{pmatrix} \frac{1}{6} \\ \frac{2}{6} \\ 0 \\ \frac{1}{6} \end{pmatrix} - \begin{pmatrix} -46/51 \\ -23/51 \\ 23/17 \\ 23/51 \end{pmatrix}$$

$$= \begin{bmatrix} 59/34 \\ 2/17 \\ 11/17 \\ -21/34 \end{bmatrix}$$

$$e_3 = \frac{q_3}{\sqrt{q_3 \cdot q_3}}$$



$$(a_3, a_3) = a_3^T M a_3$$

$$= \left( \frac{59}{34}, \frac{2}{17}, \frac{11}{17}, -\frac{21}{34} \right) \begin{pmatrix} 2 & -1 & 0 & 0 \\ -1 & 3 & 0 & 0 \\ 0 & 0 & 4 & 1 \\ 0 & 0 & 1 & 2 \end{pmatrix} \begin{matrix} 59/34 \\ 2/17 \\ 11/17 \\ -21/34 \end{matrix}$$

$$= \left( \frac{59}{34}, \frac{2}{17}, \frac{11}{17}, -\frac{21}{34} \right) \begin{pmatrix} 2 \times \frac{59}{34} - 1 \times \frac{2}{17} + 0 + 0 \\ -1 \times \frac{59}{34} + 3 \times \frac{2}{17} + 0 + 0 \\ 0 + 0 + 4 \times \frac{11}{17} + 1 \times \frac{-21}{34} \\ 0 + 0 + 1 \times \frac{11}{17} + 2 \times \frac{-21}{34} \end{pmatrix}$$

$$= \left( \frac{59}{34}, \frac{2}{17}, \frac{11}{17}, -\frac{21}{34} \right) \begin{pmatrix} 57/17 \\ -47/34 \\ 67/34 \\ -10/17 \end{pmatrix}$$

$$= \left( \frac{59}{34} \times \frac{57}{17} \right) + \left( \frac{2}{17} \times \frac{-47}{34} \right) + \left( \frac{11}{17} \times \frac{67}{34} \right) + \left( \frac{-21}{34} \times \frac{-10}{17} \right)$$

$$= \frac{4216}{578}$$

$$= \frac{124}{17}$$

(35)

Suresh babu

\_/\_/\_

2025ab05129

$$e_3 = \frac{q_3}{\sqrt{A_3 q_3}} = \frac{1}{\sqrt{124/17}} \begin{bmatrix} 59/34 \\ 2/17 \\ 11/17 \\ -21/34 \end{bmatrix}$$

Ortho normal set with respect to Inner product is

$$e_1 = \frac{1}{2\sqrt{3}} \begin{bmatrix} 1 & 2 & 0 & 1 \end{bmatrix}^T$$

$$e_2 = \sqrt{3/17} \begin{bmatrix} -2/3 & -1/3 & 1 & 1/3 \end{bmatrix}^T$$

$$e_3 = \sqrt{\frac{17}{124}} \begin{bmatrix} 59/34 & 2/17 & 11/17 & -21/34 \end{bmatrix}^T$$